Weidenbach_Book/Watched_Literals_Algorithm.thy
@@ -683,66 +683,6 @@ definition backtrack :: \<open>'v twl_st \<Rightarrow> 'v twl_st nres\<close> wh
   \<close>
 
 
-context conflict_driven_clause_learning\<^sub>W
-begin
-
-lemma no_step_skip_hd_in_conflicting:
-  assumes
-    inv_s: \<open>cdcl\<^sub>W_stgy_invariant S\<close> and
-    inv: \<open>cdcl\<^sub>W_all_struct_inv S\<close> and
-    ns: \<open>no_step skip S\<close> and
-    confl: \<open>conflicting S \<noteq> None\<close> \<open>conflicting S \<noteq> Some {#}\<close>
-  shows \<open>-lit_of (hd (trail S)) \<in># the (conflicting S)\<close>
-proof -
-  let
-    ?M = \<open>trail S\<close> and
-    ?N = \<open>init_clss S\<close> and
-    ?U = \<open>learned_clss S\<close> and
-    ?k = \<open>backtrack_lvl S\<close> and
-    ?D = \<open>conflicting S\<close>
-  obtain D where D: \<open>?D = Some D\<close>
-    using confl by (cases ?D) auto
-  have M_D: \<open>?M \<Turnstile>as CNot D\<close>
-    using inv D unfolding cdcl\<^sub>W_all_struct_inv_def cdcl\<^sub>W_conflicting_def by auto
-  then have tr: \<open>trail S \<noteq> []\<close>
-    using confl D by auto
-  obtain L M where M: \<open>?M = L # M\<close>
-    using tr by (cases \<open>?M\<close>) auto
-  have conlf_k: \<open>conflict_is_false_with_level S\<close>
-    using inv_s unfolding cdcl\<^sub>W_stgy_invariant_def by simp
-  then obtain L_k where
-    L_k: \<open>L_k \<in># D\<close> and lev_L_k: \<open>get_level ?M L_k = ?k\<close>
-    using confl D by auto
-  have dec: \<open>?k = count_decided ?M\<close>
-    using inv unfolding cdcl\<^sub>W_all_struct_inv_def cdcl\<^sub>W_M_level_inv_def by auto
-  moreover {
-    have \<open>no_dup ?M\<close>
-      using inv unfolding cdcl\<^sub>W_all_struct_inv_def cdcl\<^sub>W_M_level_inv_def by auto
-    then have \<open>-lit_of L \<notin> lits_of_l M\<close>
-      unfolding M by (auto simp: defined_lit_map lits_of_def uminus_lit_swap)
-    }
-  ultimately have L_D: \<open>lit_of L \<notin># D\<close>
-    using M_D unfolding M by (auto simp add: true_annots_true_cls_def_iff_negation_in_model
-        uminus_lit_swap)
-  show ?thesis
-  proof (cases L)
-    case (Decided L') note L' = this(1)
-    moreover have \<open>atm_of L' = atm_of L_k\<close>
-      using lev_L_k count_decided_ge_get_level[of M L_k] unfolding M dec L'
-      by (auto simp: get_level_cons_if split: if_splits)
-    then have \<open>L' = -L_k\<close>
-      using L_k L_D L' by (auto simp: atm_of_eq_atm_of)
-    then show ?thesis using L_k unfolding D M L' by simp
-  next
-    case (Propagated L' C)
-    then show ?thesis
-      using ns confl by (auto simp: skip.simps M D)
-  qed
-qed
-
-end
-
-
 lemma
   assumes confl: \<open>get_conflict S \<noteq> None\<close> \<open>get_conflict S \<noteq> Some {#}\<close> and
     w_q: \<open>clauses_to_update S = {#}\<close> and p: \<open>literals_to_update S = {#}\<close> and
